Completed verification message header
Feat: Added predicates and proofs MessageHeaderBody and MessageHeader
Feat: Added prove duality MessageHeaderBody serialize and deserialize

src/SDK/MessageHeader.dfy
@@ -163,4 +163,29 @@ module {:extern "MessageHeader"} MessageHeader {
     UInt16ToSeq(|edk.providerInfo| as uint16) + edk.providerInfo +
     UInt16ToSeq(|edk.ciphertext| as uint16)   + edk.ciphertext
   }
+
+  predicate {:opaque} SeqToHeaderBody(sequence: seq<uint8>, hb: HeaderBody)
+    requires hb.Valid()
+  {
+    exists serializedAAD | EncryptionContext.LinearSeqToMap(serializedAAD, hb.aad) ::
+      sequence == 
+        [hb.version as uint8] +
+        [hb.typ as uint8] +
+        UInt16ToSeq(hb.algorithmSuiteID as uint16) +
+        hb.messageID +
+        serializedAAD + // This field can be encrypted in multiple ways and prevents us from reusing HeaderBodyToSeq
+        EDKsToSeq(hb.encryptedDataKeys) +
+        [ContentTypeToUInt8(hb.contentType)] +
+        Reserved +
+        [hb.ivLength] +
+        UInt32ToSeq(hb.frameLength)
+  }
+
+  lemma SeqToHeaderBodyDuality(hb: HeaderBody)
+    requires hb.Valid()
+    ensures SeqToHeaderBody(HeaderBodyToSeq(hb), hb)
+  {
+    reveal HeaderBodyToSeq(), SeqToHeaderBody();
+    EncryptionContext.MapToLinearIsDualLinearSeqToMap(hb.aad);
+  }
 }
